$\frac{(-1)^{n}}{\sqrt{ n }+(-1)^{n}}=\frac{(-1)^{n}}{\sqrt{ n }}\cdot \frac{1}{1+\frac{(-1)^{n}}{\sqrt{ n }}}=\frac{(-1)^{n}}{\sqrt{ n }}\left( 1-\frac{(-1)^{n}}{\sqrt{ n }}+o\left( \frac{1}{\sqrt{ n }} \right) \right)$
$=\frac{(-1)^{n}}{\sqrt{ n }}-\left( \frac{1}{n}+o\left( \frac{1}{n} \right) \right)$
- chuỗi $\sum_{n=1}^{\infty} \frac{(-1)^{n}}{\sqrt{ n }}$ hội tụ theo leibnitz
- chuỗi $\sum_{n=1}^{\infty}\left( \frac{1}{n}+o\left( \frac{1}{n} \right) \right)$ phân kỳ do $\lim_{ n \to \infty } \frac{\frac{1}{n}+o\left( \frac{1}{n} \right)}{\frac{1}{n}}=1$ và $\sum_{n=1}^{\infty} \frac{1}{n}$ phân kỳ


$2x^{2}y'=y^{3}+xy$